src/Assembly/GF25519.v
@@ -9,6 +9,9 @@ Module GF25519.
   Definition bits: nat := 64.
   Definition width: Width bits := W64.
 
+  Instance ZE : Evaluable Z := @ZEvaluable bits.
+  Existing Instance ZE.
+
   Fixpoint makeBoundList {n} k (b: @BoundedWord n) :=
     match k with
     | O => nil
@@ -17,9 +20,9 @@ Module GF25519.
 
   Section DefaultBounds.
     Import ListNotations.
-    Local Notation rr exp := (range N 0%N (2^exp + 2^exp/10)%N).
+    Local Notation rr exp := (2^exp + 2^exp/10)%N.
 
-    Definition feBound: list (Range N) :=
+    Definition feBound: list N :=
       [rr 26; rr 27; rr 26; rr 27; rr 26;
        rr 27; rr 26; rr 27; rr 26; rr 27].
   End DefaultBounds.
@@ -45,8 +48,7 @@ Module GF25519.
         Eval cbv beta delta [fe25519 add mul sub Let_In] in add.
 
     Definition ge25519_add' (P Q: @interp_type Z FE) :
-        { r: @HL.expr Z (@interp_type Z) FE
-        | HL.interp (E := ZEvaluable) (t := FE) r = ge25519_add_expr P Q }.
+        { r: @HL.expr Z FE | HL.Interp (t := FE) r = ge25519_add_expr P Q }.
     Proof.
       vm_compute in P, Q; repeat
         match goal with
@@ -62,9 +64,8 @@ Module GF25519.
       cbv beta delta [ge25519_add_expr].
 
       let R := HL.rhs_of_goal in
-      let X := HL.reify (@interp_type Z) R in
-      transitivity (HL.interp (E := ZEvaluable) (t := ResultType) X);
-        [reflexivity|].
+      let X := HL.Reify R in
+      transitivity (HL.Interp (t := ResultType) X); [reflexivity|].
 
       cbv iota beta delta [
             interp_type interp_binop HL.interp
@@ -75,16 +76,11 @@ Module GF25519.
     Definition ge25519_add (P Q: @interp_type Z ResultType) :=
         proj1_sig (ge25519_add' P Q).
 
-    Definition hlProg'': NAry 20 Z (@HL.expr Z (@interp_type Z) ResultType) :=
+    Definition hlProg': NAry 20 Z (@HL.Expr Z ResultType) :=
         liftFE (fun p => (liftFE (fun q => ge25519_add p q))).
 
-    Definition hlProg': NAry 20 Z (@HL.expr Z (@LL.arg Z Z) ResultType).
-        refine (liftN (HLConversions.mapVar _ _) hlProg''); intro t;
-        [ refine LL.uninterp_arg | refine LL.interp_arg ].
-    Defined.
-
-    Definition hlProg: NAry 20 Z (@HL.expr Z (@LL.arg Z Z) ResultType) :=
-      Eval vm_compute in hlProg'.
+    Definition hlProg: NAry 20 Z (@CompileHL.Expr' Z ResultType) :=
+      Eval vm_compute in (liftN (fun P => (fun T => P (@LL.arg Z T))) hlProg').
   End AddExpr.
 
   Module SubExpr <: Expression.
@@ -234,16 +230,8 @@ Module GF25519.
     Definition ge25519_opp (P: @interp_type Z ResultType) :=
         proj1_sig (ge25519_opp' P).
 
-    Definition hlProg'': NAry 10 Z (@HL.expr Z (@interp_type Z) ResultType) :=
+    Definition hlProg: NAry 10 Z (@HL.expr Z (@interp_type Z) ResultType) :=
         liftFE (fun p => ge25519_opp p).
-
-    Definition hlProg': NAry 10 Z (@HL.expr Z (@LL.arg Z Z) ResultType).
-        refine (liftN (HLConversions.mapVar _ _) hlProg''); intro t;
-        [ refine LL.uninterp_arg | refine LL.interp_arg ].
-    Defined.
-
-    Definition hlProg: NAry 10 Z (@HL.expr Z (@LL.arg Z Z) ResultType) :=
-      Eval vm_compute in hlProg'.
   End OppExpr.
 
   Module Add := Pipeline AddExpr.
